CFPrim.v
@@ -5,6 +5,8 @@ Require Export LibInt LibArray CFSpec CFPrint.
 (* todo: move *)
 Implicit Arguments list_sub [[A]].
 
+(* todo: move *)
+
 Hint Resolve (0%nat) : typeclass_instances.
 Hint Resolve (0%Z) : typeclass_instances.
 Hint Resolve @nil : typeclass_instances.
@@ -20,78 +22,17 @@ Ltac inhab :=
     | apply @arbitrary; eauto 10 with typeclass_instances ].
 
 Instance inhabited_Z : Inhabited Z.
-Admitted. (* todo --trivial *)
+Admitted. (* todo -- trivial, use 0%Z *)
 
-
+(* todo: move *)
 Global Opaque heap_is_empty hdata heap_is_single heap_is_empty_st.
 Global Opaque Zplus.
 
 
 (********************************************************************)
-(** Pure Representation for base types *)
-
-
-Hint Extern 1 (@rep _ _ _ _ _) => simpl.
-
-Hint Resolve @rep_unique : rep.
-
-Ltac prove_rep := 
-  fequals_rec; 
-  try match goal with |- @eq (?T ?A) _ _ => let U := fresh in sets U:(T A) end;
-  intuition eauto with rep.
-  (* todo : appliquer directement rep_unique sur les buts ? *)
-
-Instance int_rep : Rep int int.
-Proof. apply (Build_Rep eq). congruence. Defined.
-
-Instance bool_rep : Rep bool bool.
-Proof. apply (Build_Rep eq). congruence. Defined.
-
-Instance list_rep : forall `{Rep a A}, Rep (list a) (list A).
-Proof.
-  intros. apply (Build_Rep (fun l L => Forall2 rep l L)).
-  induction x; introv H1 H2; inverts H1; inverts H2; prove_rep. 
-Defined.
-
-Lemma list_rep_cons : forall `{Rep a A} l L x X,
-  rep l L -> rep x X -> rep (x::l) (X::L).
-Proof. intros. constructors~. Qed.
-
-Hint Resolve @list_rep_cons.
-
-Instance prod_rep : forall `{Rep a1 A1} `{Rep a2 A2},
-  Rep (a1 * a2) (A1 * A2).
-Proof.
-  intros. apply (Build_Rep (fun p P => match p,P with 
-   (x,y),(X,Y) => rep x X /\ rep y Y end)).
-  intros [x1 x2] [X1 X2] [Y1 Y2] H1 H2; prove_rep.
-Defined.
-
-Instance option_rep : forall `{Rep a A},
-  Rep (option a) (option A).
-Proof.
-  intros. apply (Build_Rep (fun o O => match o,O with 
-    | None, None => True
-    | Some x, Some X => rep x X
-    | _,_ => False end)).
-  intros [x|] [X|] [Y|] H1 H2; prove_rep.
-Defined.
-
-Hint Extern 1 (@rep (list _) _ _ _ _) => simpl.
-Hint Extern 1 (@rep (prod _ _) _ _ _ _) => simpl.
-Hint Extern 1 (@rep (option _) _ _ _ _) => simpl.
-
-
-(* todo: move *)
-Definition nref := loc.
-Parameter null : loc.
-Parameter ml_is_null : val.
-
-
-(********************************************************************)
 (** Imperative Representation for base types *)
 
-Definition htype A a := A -> a -> hprop.
+Transparent hdata. (* TODO: use hdata_simpl instead *)
 
 
 (*------------------------------------------------------------------*)
@@ -113,17 +54,22 @@ Implicit Arguments Id_unfocus [A].
 
 
 (*------------------------------------------------------------------*)
-(* ** Void and Any *)
+(* ** Any *)
 
-Definition Void {a A} (v:a) (V:A) := 
-  []. (* todo: used? *)
+(** [x ~> Any tt] describes the fact that x points towards something
+    whose value is not relevant. In other words, the model is unit.
+    Note: [[True]] is used in place of [[]] to avoid confusing tactics. *)
 
 Definition Any {A:Type} (X:unit) (x:A) := 
-  [True]. (* should not be [] otherwise tactics bug *)
-
+  [True].
+ 
 
 (*------------------------------------------------------------------*)
 (* ** References *)
+
+(* TODO: ideally, references should be treated simply
+   as a record with a single field, so the following
+   material would be generated automatically. *)
 
 Definition Ref a A (T:htype A a) (V:A) (l:loc) :=
   Hexists v, heap_is_single l v \* v ~> T V.
@@ -132,12 +78,7 @@ Notation "l '~~>' v" := (l ~> Ref Id v)
   (at level 32, no associativity).
 Notation "'~~>' v" := (~> Ref Id v)
   (at level 32, no associativity) : heap_scope.
-(*
-Lemma focus_ref_core : forall (l:loc) a A (T:htype A a) V,
-  l ~> Ref T V ==> Hexists v, l> v \* v ~> T V.
-Proof. auto. Qed.
-*)
-Transparent hdata.
+
 Lemma focus_ref : forall (l:loc) a A (T:htype A a) V,
   l ~> Ref T V ==> Hexists v, l ~~> v \* v ~> T V.
 Proof. intros. unfold Ref, hdata. unfold Id. hextract.
@@ -150,11 +91,8 @@ Proof. intros. unfold Ref. hdata_simpl. hextract. hsimpl. subst~. Qed.
 Axiom focus_ref_null : forall a A (T:htype A a) V,
   null ~> Ref T V ==> [False]. (* todo *)
 
-Opaque Ref.
+Global Opaque Ref.
 
-
-
-   (*--todo: Record ref A := { content : A }. *)
 
 (*------------------------------------------------------------------*)
 (* ** Tuple 2 *)
@@ -170,7 +108,7 @@ Lemma unfocus_tup2 : forall a1 (x1:a1) a2 (x2:a2) A1 A2 (T1:htype A1 a1) (T2:hty
   x1 ~> T1 V1 \* x2 ~> T2 V2 ==> (x1,x2) ~> Tup2 T1 T2 (V1,V2).
 Proof. intros. unfold Tup2. hdata_simpl. auto. Qed.
 
-Opaque Tup2.
+Global Opaque Tup2.
 
 (*------------------------------------------------------------------*)
 (* ** Tuple 3 *)
@@ -186,93 +124,7 @@ Lemma unfocus_tup3 : forall a1 (x1:a1) a2 (x2:a2) a3 (x3:a3) A1 A2 A3 (T1:htype 
   x1 ~> T1 V1 \* x2 ~> T2 V2 \* x3 ~> T3 V3 ==> (x1,x2,x3) ~> Tup3 T1 T2 T3 (V1,V2,V3).
 Proof. intros. unfold Tup3. hdata_simpl. auto. Qed.
 
-Opaque Tup3.
-
-(*------------------------------------------------------------------*)
-(* ** Ref-Tuple 3  -- todo ?
-
-Definition RefTup3 A1 A2 A3 a1 a2 a3 (T1:A1->a1->hprop) (T2:A2->a2->hprop) (T3:A3->a3->hprop) P l :=
-  l ~> Ref (Tup3 T1 T2 T3) P.
-
-Lemma focus_reftup3 : forall (l:loc) a1 a2 a3 A1 A2 A3 (T1:htype A1 a1) (T2:htype A2 a2) (T3:A3->a3->hprop) V1 V2 V3,
-  l ~> RefTup3 T1 T2 T3 (V1,V2,V3) ==> Hexists (x1:a1) (x2:a2) (x3:a3),
-  l ~> Ref Id (x1,x2,x3) \* x1 ~> T1 V1 \* x2 ~> T2 V2 \* x3 ~> T3 V3.
-Proof.
-  intros. unfold RefTup3. hdata_simpl. hchange (@focus_ref l). hextract as. 
-  intros p [[x1 x2] x3] H. hchange (focus_tup3 p). destruct p as [[y1 y2] y3].
-  inversions H. hsimpl~. 
-Qed.
-
-Lemma unfocus_reftup3 : forall (l:loc) a1 (x1:a1) a2 (x2:a2) a3 (x3:a3) A1 A2 A3 (T1:htype A1 a1) (T2:htype A2 a2) (T3:A3->a3->hprop) V1 V2 V3,
-  l ~> Ref Id (x1,x2,x3) \* x1 ~> T1 V1 \* x2 ~> T2 V2 \* x3 ~> T3 V3 ==>
-  l ~> RefTup3 T1 T2 T3 (V1,V2,V3).
-Proof.
-  intros. unfold RefTup3. hdata_simpl. hchange (unfocus_tup3 x1 x2 x3). 
-  hchange (@unfocus_ref l _ (x1,x2,x3)). hsimpl.
-Qed.
-
-Opaque RefTup3.
-*)
-
-(*------------------------------------------------------------------*)
-(* ** Record 2 *)
-
-Definition Ref2 A1 A2 a1 a2 (T1:A1->a1->hprop) (T2:A2->a2->hprop) (V1:A1) (V2:A2) l :=
-  l ~> Ref (Tup2 T1 T2) (V1,V2).
-
-Lemma focus_ref2 : forall (l:loc) a1 a2 A1 A2 (T1:htype A1 a1) (T2:htype A2 a2) V1 V2,
-  l ~> Ref2 T1 T2 V1 V2 ==> Hexists (x1:a1) (x2:a2),
-  l ~> Ref Id (x1,x2) \* x1 ~> T1 V1 \* x2 ~> T2 V2 .
-Proof.
-  intros. unfold Ref2. hdata_simpl. hchange (@focus_ref l).
-  hextract as [x1 x2]. hchange (focus_tup2 (x1,x2)). hsimpl.
-Qed.
-
-Lemma unfocus_ref2 : forall (l:loc) a1 (x1:a1) a2 (x2:a2) A1 A2 (T1:htype A1 a1) (T2:htype A2 a2) V1 V2,
-  l ~> Ref Id (x1,x2) \* x1 ~> T1 V1 \* x2 ~> T2 V2 ==>
-  l ~> Ref2 T1 T2 V1 V2.
-Proof.
-  intros. unfold Ref2. hdata_simpl. hchange (unfocus_tup2 x1 x2). 
-  hchange (@unfocus_ref l _ (x1,x2)). hsimpl.
-Qed.
-
-Lemma focus_ref2_null : forall a1 a2 A1 A2 (T1:htype A1 a1) (T2:htype A2 a2) V1 V2,
-  null ~> Ref2 T1 T2 V1 V2 ==> [False]. 
-Proof.
-  intros. unfold hdata, Ref2. hchange focus_ref_null. hsimpl. 
-Qed.
-
-Opaque Ref2.
-
-(*------------------------------------------------------------------*)
-(* ** Record 3 *)
-
-Definition Ref3 A1 A2 A3 a1 a2 a3 (T1:A1->a1->hprop) (T2:A2->a2->hprop) (T3:A3->a3->hprop) (V1:A1) (V2:A2) (V3:A3) l :=
-  l ~> Ref (Tup3 T1 T2 T3) (V1,V2,V3).
-
-Lemma focus_ref3 : forall (l:loc) a1 a2 a3 A1 A2 A3 (T1:htype A1 a1) (T2:htype A2 a2) (T3:A3->a3->hprop) V1 V2 V3,
-  l ~> Ref3 T1 T2 T3 V1 V2 V3 ==> Hexists (x1:a1) (x2:a2) (x3:a3),
-  l ~> Ref Id (x1,x2,x3) \* x1 ~> T1 V1 \* x2 ~> T2 V2 \* x3 ~> T3 V3.
-Proof.
-  intros. unfold Ref3. hdata_simpl. hchange (@focus_ref l).
-  hextract as [[x1 x2] x3]. hchange (focus_tup3 (x1,x2,x3)). hsimpl.
-Qed.
-
-Lemma unfocus_ref3 : forall (l:loc) a1 (x1:a1) a2 (x2:a2) a3 (x3:a3) A1 A2 A3 (T1:htype A1 a1) (T2:htype A2 a2) (T3:A3->a3->hprop) V1 V2 V3,
-  l ~> Ref Id (x1,x2,x3) \* x1 ~> T1 V1 \* x2 ~> T2 V2 \* x3 ~> T3 V3 ==>
-  l ~> Ref3 T1 T2 T3 V1 V2 V3.
-Proof.
-  intros. unfold Ref3. hdata_simpl. hchange (unfocus_tup3 x1 x2 x3). 
-  hchange (@unfocus_ref l _ (x1,x2,x3)). hsimpl.
-Qed.
-
-Lemma focus_ref3_null : forall a1 a2 a3 A1 A2 A3 (T1:htype A1 a1) (T2:htype A2 a2) (T3:htype A3 a3) V1 V2 V3,
-  null ~> Ref3 T1 T2 T3 V1 V2 V3 ==> [False]. 
-Proof.
-  intros. unfold hdata, Ref3. hchange focus_ref_null. hsimpl. 
-Qed.
-
-Opaque Ref3.
+Global Opaque Tup3.
 
 
 (*------------------------------------------------------------------*)
@@ -326,7 +178,7 @@ Proof.
   intros. simpl. hdata_simpl. hsimpl.
 Qed.
 
-Opaque List.
+Global Opaque List.
 
 
 (*------------------------------------------------------------------*)
@@ -382,15 +234,17 @@ Proof.
   intros. simpl. hdata_simpl. hchange (@unfocus_ref2 l _ x _ l'). hsimpl.
 Qed.
 
-Opaque MList.
+Global Opaque MList.
 
 Implicit Arguments unfocus_mnil [ ].
 Implicit Arguments unfocus_mcons [ a A ].
 Implicit Arguments focus_mcons [ a A ].
 
+
 (*------------------------------------------------------------------*)
 (* ** MListsSeg *)
-(*--todo: define MList as MListSeg null *)
+
+(* TODO: define MList as MListSeg null *)
 
 Fixpoint MListSeg (e:loc) A a (T:A->a->hprop) (L:list A) (l:loc) : hprop :=
   match L with
@@ -455,10 +309,198 @@ Axiom mlistseg_to_mlist : forall (l:loc) a A (T:htype A a) L,
    l ~> MListSeg null T L ==> l ~> MList T L.
 Axiom mlist_to_mlistseg : forall (l:loc) a A (T:htype A a) L,
    l ~> MList T L ==> l ~> MListSeg null T L.
-(*todo*)
+(* --todo-- *)
 
-Opaque MListSeg.
+Global Opaque MListSeg.
 
+
+
+(************************************************************)
+(** Axiomatic specification of the primitive functions *)
+
+(** Pointer comparison *)
+
+Parameter ml_phy_eq : func.
+Parameter ml_phy_eq_spec : Pure ml_phy_eq x y >> = (x '= y :> loc).
+Hint Extern 1 (RegisterSpec ml_phy_eq) => Provide ml_phy_eq_spec.
+
+Parameter ml_phy_neq : func.
+Parameter ml_phy_neq_spec : Pure ml_phy_neq x y >> = (x '<> y :> loc).
+Hint Extern 1 (RegisterSpec ml_phy_neq) => Provide ml_phy_neq_spec.
+
+(** Arithmetic *)
+
+Parameter ml_plus : func.
+Parameter ml_plus_spec : Pure ml_plus x y >> = (x + y)%Z.
+Hint Extern 1 (RegisterSpec ml_plus) => Provide ml_plus_spec.
+
+Parameter ml_minus : func.
+Parameter ml_minus_spec : Pure ml_minus x y >> = (x - y)%Z.
+Hint Extern 1 (RegisterSpec ml_minus) => Provide ml_minus_spec.
+
+Parameter ml_eqb : func.
+Parameter ml_eqb_int_spec : Pure ml_eqb (x:int) (y:int) >> = (x '= y).
+Hint Extern 1 (RegisterSpec ml_eqb) => Provide ml_eqb_int_spec.
+
+Parameter ml_leq : func.
+Parameter ml_leq_spec : Pure ml_leq x y >> = (x <= y)%I.
+Hint Extern 1 (RegisterSpec ml_leq) => Provide ml_leq_spec.
+
+Parameter ml_geq : func.
+Parameter ml_geq_spec : Pure ml_geq x y >> = (x >= y)%I.
+Hint Extern 1 (RegisterSpec ml_geq) => Provide ml_geq_spec.
+
+Parameter ml_lt : func.
+Parameter ml_lt_spec : Pure ml_lt x y >> = (x < y)%I.
+Hint Extern 1 (RegisterSpec ml_lt) => Provide ml_lt_spec.
+
+Parameter ml_gt : func.
+Parameter ml_gt_spec : Pure ml_gt x y >> = (x > y)%I.
+Hint Extern 1 (RegisterSpec ml_gt) => Provide ml_gt_spec.
+
+Parameter ml_and : func.
+Parameter ml_and_spec : Pure ml_and x y >> = (x && y).
+Hint Extern 1 (RegisterSpec ml_and) => Provide ml_and_spec.
+
+Parameter ml_or : func.
+Parameter ml_or_spec : Pure ml_or x y >> = (x || y).
+Hint Extern 1 (RegisterSpec ml_and) => Provide ml_or_spec.
+ 
+  (*todo:*)
+  Parameter ml_min_int : int.
+  Parameter ml_max_int : int.
+  Parameter ml_rand_int : func.
+
+(** Pairs *)
+
+Parameter ml_fst : func.
+Parameter ml_fst_spec : forall a1 a2,
+  Spec ml_fst (p:a1*a2) |R>> 
+    pure R (= fst p).
+Hint Extern 1 (RegisterSpec ml_fst) => Provide ml_fst_spec.
+
+Parameter ml_snd : func.
+Parameter ml_snd_spec : forall a1 a2,
+  Spec ml_snd (p:a1*a2) |R>> 
+    pure R (= snd p).
+Hint Extern 1 (RegisterSpec ml_snd) => Provide ml_snd_spec.
+
+(** References *)
+
+Parameter ml_ref : func.
+Parameter ml_get : func.
+Parameter ml_set : func.
+Parameter ml_incr : func.
+Parameter ml_decr : func.
+
+Parameter ml_ref_spec : forall a,
+  Spec ml_ref (v:a) |R>> 
+    R [] (~~> v).
+
+Parameter ml_get_spec : forall a,
+  Spec ml_get (l:loc) |R>> 
+    forall (v:a), keep R (l ~~> v) (\=v).
+
+Parameter ml_set_spec : forall a,
+  Spec ml_set (l:loc) (v:a) |R>> 
+    forall (v':a), R (l ~> Ref Id v') (# l ~> Ref Id v).
+
+Parameter ml_incr_spec : 
+  Spec ml_incr (l:loc) |R>> 
+    forall n, R (l ~~> n) (# l ~~> (n+1)).
+ 
+Parameter ml_decr_spec : 
+  Spec ml_decr (l:loc) |R>> 
+    forall n, R (l ~~> n) (# l ~~> (n-1)).
+
+Hint Extern 1 (RegisterSpec ml_ref) => Provide ml_ref_spec.
+Hint Extern 1 (RegisterSpec ml_get) => Provide ml_get_spec.
+Hint Extern 1 (RegisterSpec ml_set) => Provide ml_set_spec.
+Hint Extern 1 (RegisterSpec ml_incr) => Provide ml_incr_spec.
+Hint Extern 1 (RegisterSpec ml_decr) => Provide ml_decr_spec.
+
+(** Strong References *) (* TODO: unify with normal ref? *)
+
+Parameter ml_sset : func.
+Parameter ml_sset_spec : forall a a',
+  Spec ml_sset (l:loc) (v:a) |R>> 
+    forall (v':a'), R (l ~~> v') (# l ~~> v).
+Hint Extern 1 (RegisterSpec ml_sset) => Provide ml_sset_spec.
+
+(** List *) 
+
+Parameter ml_list_iter : func.
+
+  (* TODO *)
+
+(** Arrays *)
+
+Parameter ml_array_make : func.
+Parameter ml_array_get : func.
+Parameter ml_array_set : func.
+Parameter ml_array_init : func.
+Parameter ml_array_length : func.
+
+Parameter Array : forall a A (T:htype A a) (M:array A) (l:loc), hprop.
+
+Require Import LibBag.
+
+Parameter ml_array_make_spec : forall a,
+  Spec ml_array_make (n:int) (v:a) |R>> 
+     R [] (~> Array Id (LibArray.make n v)).
+     (* (fun l => Hexists t, l ~> Array Id t \* [t = array_make n v]). *)
+
+Parameter ml_array_get_spec : forall a,
+  Spec ml_array_get (l:loc) (i:int) |R>> 
+    forall `{Inhab a} (t:array a), index t i ->
+    keep R (l ~> Array Id t) (\= t\(i)).
+
+Parameter ml_array_set_spec : forall a,
+  Spec ml_array_set (l:loc) (i:int) (v:a) |R>> 
+    forall (t:array a), index t i -> 
+    R (l ~> Array Id t) (# l ~> Array Id (t\(i:=v))).
+      (* (# Hexists t', l ~> Array Id t' \* [t' = t\(i:=v)]).*)
+
+Parameter ml_array_length_spec : forall a,
+  Spec ml_array_length (l:loc) |R>> forall (t:array a),
+    keep R (l ~> Array Id t) (\= LibArray.length t).
+
+Hint Extern 1 (RegisterSpec ml_array_make) => Provide ml_array_make_spec.
+Hint Extern 1 (RegisterSpec ml_array_get) => Provide ml_array_get_spec.
+Hint Extern 1 (RegisterSpec ml_array_set) => Provide ml_array_set_spec.
+Hint Extern 1 (RegisterSpec ml_array_length) => Provide ml_array_length_spec.
+
+
+
+(********************************************************************)
+(** IO manipulations *)
+
+(*------------------------------------------------------------------*)
+(* ** IO representation *)
+
+Parameter Channel : forall (L:list dynamic) (l:loc), hprop.
+
+Notation "l ~>> L" := (l ~> Channel L)
+  (at level 32, no associativity).
+
+Parameter stdin : loc.
+Parameter stdout : loc.
+
+
+(*------------------------------------------------------------------*)
+(* ** IO primitives *)
+
+Parameter ml_read_int : func.
+Parameter ml_read_int_spec :
+  Spec ml_read_int () |R>> forall L (n:int),
+    R (stdin ~>> (dyn n::L)) (\=n \*+ stdin ~>> L).
+Hint Extern 1 (RegisterSpec ml_read_int) => Provide ml_read_int_spec.
+
+Parameter ml_print_int : func.
+Parameter ml_print_int_spec :
+  Spec ml_print_int (n:int) |R>> forall L,
+    R (stdout ~>> L) (# stdout ~>> L & (dyn n)).
+Hint Extern 1 (RegisterSpec ml_print_int) => Provide ml_print_int_spec.
 
 
 (*------------------------------------------------------------------*)
@@ -488,276 +530,3 @@ Hint Rewrite list_dyn_cons : rew_list.
 Hint Rewrite list_dyn_last : rew_app.
 Hint Rewrite list_dyn_last : rew_map.
 Hint Rewrite list_dyn_last : rew_list.
-
-
-
-(************************************************************)
-(** Axiomatic specification of the primitive functions *)
-
-
-(* todo: move *)
-Notation "x ''=' y :> A" := (istrue (@eq A x y))
-  (at level 70, y at next level, only parsing) : comp_scope.
-Notation "x ''<>' y :> A" := (istrue (~ (@eq A x y)))
-  (at level 69, y at next level, only parsing) : comp_scope.
-
-
-(* todo?
-Parameter ml_is_null_spec : 
-  Spec ml_is_null l |R>> R [] (\[ bool_of (l = null)]).
-
-Hint Extern 1 (RegisterSpec ml_is_null) => Provide ml_is_null_spec.
- *)
-
-
-(** Pointers *)
-
-Parameter ml_phy_eq : val.
-Parameter ml_phy_eq_spec : Pure ml_phy_eq x y >> = (x '= y :> loc).
-Hint Extern 1 (RegisterSpec ml_phy_eq) => Provide ml_phy_eq_spec.
-
-Parameter ml_phy_neq : val.
-Parameter ml_phy_neq_spec : Pure ml_phy_neq x y >> = (x '<> y :> loc).
-Hint Extern 1 (RegisterSpec ml_phy_neq) => Provide ml_phy_neq_spec.
-
-(** Arithmetic *)
-
-Parameter ml_plus : val.
-Parameter ml_plus_spec : Pure ml_plus x y >> = (x + y)%Z.
-Hint Extern 1 (RegisterSpec ml_plus) => Provide ml_plus_spec.
-
-Parameter ml_minus : val.
-Parameter ml_minus_spec : Pure ml_minus x y >> = (x - y)%Z.
-Hint Extern 1 (RegisterSpec ml_minus) => Provide ml_minus_spec.
-
-Parameter ml_eqb : val.
-Parameter ml_eqb_int_spec : Pure ml_eqb (x:int) (y:int) >> = (x == y).
-Hint Extern 1 (RegisterSpec ml_eqb) => Provide ml_eqb_int_spec.
-
-Parameter ml_leq : val.
-Parameter ml_leq_spec : Pure ml_leq x y >> = (x <= y)%I.
-Hint Extern 1 (RegisterSpec ml_leq) => Provide ml_leq_spec.
-
-Parameter ml_geq : val.
-Parameter ml_geq_spec : Pure ml_geq x y >> = (x >= y)%I.
-Hint Extern 1 (RegisterSpec ml_geq) => Provide ml_geq_spec.
-
-Parameter ml_lt : val.
-Parameter ml_lt_spec : Pure ml_lt x y >> = (x < y)%I.
-Hint Extern 1 (RegisterSpec ml_lt) => Provide ml_lt_spec.
-
-Parameter ml_gt : val.
-Parameter ml_gt_spec : Pure ml_gt x y >> = (x > y)%I.
-Hint Extern 1 (RegisterSpec ml_gt) => Provide ml_gt_spec.
-
-Parameter ml_and : val.
-Parameter ml_and_spec : Pure ml_and x y >> = (x && y).
-Hint Extern 1 (RegisterSpec ml_and) => Provide ml_and_spec.
-
-Parameter ml_or : val.
-Parameter ml_or_spec : Pure ml_or x y >> = (x || y).
-Hint Extern 1 (RegisterSpec ml_and) => Provide ml_or_spec.
-
-Parameter ml_min_int : int.
-Parameter ml_max_int : int.
-Parameter ml_rand_int : val.
-
-(** Pairs *)
-
-Parameter ml_fst : val.
-Parameter ml_fst_spec : forall a1 a2,
-  Spec ml_fst (p:a1*a2) |R>> 
-    pure R (= fst p).
-Hint Extern 1 (RegisterSpec ml_fst) => Provide ml_fst_spec.
-
-Parameter ml_snd : val.
-Parameter ml_snd_spec : forall a1 a2,
-  Spec ml_snd (p:a1*a2) |R>> 
-    pure R (= snd p).
-Hint Extern 1 (RegisterSpec ml_snd) => Provide ml_snd_spec.
-
-(** IO *)
-
-Parameter Channel : forall (L:list dynamic) (l:loc), hprop.
-
-Notation "l ~>> L" := (l ~> Channel L)
-  (at level 32, no associativity).
-
-Parameter stdin : loc.
-Parameter stdout : loc.
-
-Parameter ml_read_int : val.
-Parameter ml_read_int_spec :
-  Spec ml_read_int () |R>> forall L (n:int),
-    R (stdin ~>> (dyn n::L)) (\=n \*+ stdin ~>> L).
-Hint Extern 1 (RegisterSpec ml_read_int) => Provide ml_read_int_spec.
-
-Parameter ml_print_int : val.
-Parameter ml_print_int_spec :
-  Spec ml_print_int (n:int) |R>> forall L,
-    R (stdout ~>> L) (# stdout ~>> L & (dyn n)).
-Hint Extern 1 (RegisterSpec ml_print_int) => Provide ml_print_int_spec.
-
-
-(** References *)
-
-Parameter ml_ref : val.
-Parameter ml_get : val.
-Parameter ml_set : val.
-Parameter ml_incr : val.
-Parameter ml_decr : val.
-
-Parameter ml_ref_spec : forall a,
-  Spec ml_ref (v:a) |R>> 
-    R [] (~~> v).
-
-Parameter ml_get_spec : forall a,
-  Spec ml_get (l:loc) |R>> 
-    forall (v:a), keep R (l ~~> v) (\=v).
-
-Parameter ml_set_spec : forall a,
-  Spec ml_set (l:loc) (v:a) |R>> 
-    forall (v':a), R (l ~> Ref Id v') (# l ~> Ref Id v).
-
-Parameter ml_incr_spec : 
-  Spec ml_incr (l:loc) |R>> 
-    forall n, R (l ~~> n) (# l ~~> (n+1)).
- 
-Parameter ml_decr_spec : 
-  Spec ml_decr (l:loc) |R>> 
-    forall n, R (l ~~> n) (# l ~~> (n-1)).
-
-Hint Extern 1 (RegisterSpec ml_ref) => Provide ml_ref_spec.
-Hint Extern 1 (RegisterSpec ml_get) => Provide ml_get_spec.
-Hint Extern 1 (RegisterSpec ml_set) => Provide ml_set_spec.
-Hint Extern 1 (RegisterSpec ml_incr) => Provide ml_incr_spec.
-Hint Extern 1 (RegisterSpec ml_decr) => Provide ml_decr_spec.
-
-(** Strong References --todo unify ? *)
-Parameter ml_sset : val.
-Parameter ml_sset_spec : forall a a',
-  Spec ml_sset (l:loc) (v:a) |R>> 
-    forall (v':a'), R (l ~~> v') (# l ~~> v).
-Hint Extern 1 (RegisterSpec ml_sset) => Provide ml_sset_spec.
-
-
-(** Derived specifications for references *)
-
-Lemma ml_ref_spec_linear : forall A a,
-  Spec ml_ref (v:a) |R>> forall (V:A) (T:htype A a),
-    R (v ~> T V) (~> Ref T V).
-Proof.
-  intros. applys spec_weaken_1 ml_ref_spec.
-  intros_all. unfolds rel_le, pred_le. auto*. (* xisspec *)
-  introv L M. intros.
-  applys local_wframe. auto. eauto.
-  hsimpl. intros l.
-  hchange~ (@unfocus_ref l _ x1). hsimpl.
-Qed.
-
-(*
-Lemma ml_get_spec_linear : forall A a,
-  Spec ml_get (l:loc) |R>> 
-    forall (V:A) (T:htype A a), 
-    R (l ~> Ref T V) (fun v => l ~> RefOn v \* T V v).
-Proof.
-  intros. applys spec_weaken_1 ml_get_spec.
-  intros_all. unfolds rel_le, pred_le. auto*. (* xisspec *)
-  introv L M. intros. unfold hdata.
-  unfold Ref. hclean. intros v.
-  specializes M v.
-  applys local_wframe. auto. eauto. hsimpl.
-  intros l. (* unfold starpost. todo: as notation *) 
-  simpl. unfold hdata.
-  (* todo: tactic hsimpl_left should do it *)
-  hsimpl. apply heap_extract_prop. intro_subst. auto.
-Qed.
-*)
-
-(** List *)
-
-Parameter ml_list_iter : val.
-
-(** Arrays *)
-
-Parameter ml_array_make : val.
-Parameter ml_array_get : val.
-Parameter ml_array_set : val.
-Parameter ml_array_init : val.
-Parameter ml_array_length : val.
-
-
-(*
-Definition ArrayOn A (v:array A) (l:loc) : hprop.
- (* := l ~~> v.*)
-*)
-
-Axiom array_make : forall A (n:int) (v:A), array A.
-
-
-
-Parameter Array : forall a A (T:htype A a) (M:array A) (l:loc), hprop.
-
-Require Import LibBag.
-
-Parameter ml_array_make_spec : forall a,
-  Spec ml_array_make (n:int) (v:a) |R>> 
-     R [] (~> Array Id (array_make n v)).
-     (* (fun l => Hexists t, l ~> Array Id t \* [t = array_make n v]). *)
-
-Parameter ml_array_get_spec : forall a,
-  Spec ml_array_get (l:loc) (i:int) |R>> 
-    forall `{Inhab a} (t:array a), index t i ->
-    keep R (l ~> Array Id t) (\= t\(i)).
-
-Parameter ml_array_set_spec : forall a,
-  Spec ml_array_set (l:loc) (i:int) (v:a) |R>> 
-    forall (t:array a), index t i -> 
-    R (l ~> Array Id t) (# l ~> Array Id (t\(i:=v))).
-      (* (# Hexists t', l ~> Array Id t' \* [t' = t\(i:=v)]).*)
-
-Parameter ml_array_length_spec : forall a,
-  Spec ml_array_length (l:loc) |R>> forall (t:array a),
-    keep R (l ~> Array Id t) (\= LibArray.length t).
-
-Hint Extern 1 (RegisterSpec ml_array_make) => Provide ml_array_make_spec.
-Hint Extern 1 (RegisterSpec ml_array_get) => Provide ml_array_get_spec.
-Hint Extern 1 (RegisterSpec ml_array_set) => Provide ml_array_set_spec.
-Hint Extern 1 (RegisterSpec ml_array_length) => Provide ml_array_length_spec.
-
-(*
-
-Class Dup a A (T:htype A a) : Prop := { 
-  dup : forall X x, T X x ==> [] }.
-*)
-
-
-Global Opaque Ref.
-
-
-(*
-let incr r = 
-   r := !r + 1
-
-let not b =
-  if b then false else true
-
-let fst (x,y) = x
-let snd (x,y) = y
-*)
-
-
-
-
-
-(*
-
-Lemma focus_mcons : forall (l:loc) A (X:A) (L':list A),
-  (l ~> Mlist (X::L')) ==>
-  Hexists l', (l ~~> (X,l')) \* (l' ~> Mlist L').
-Proof.
-  intros. simpl. hdata_simpl. auto. 
-Qed.
-*)
-
-
